01Source/SourceLanguage.thy
@@ -1,0 +1,98 @@
+theory SourceLanguage
+  imports "../00Utils/Variable" "../00Utils/Utils"
+begin
+
+section \<open>Source Language\<close>
+
+text \<open>We now define our source language. It consists of the untyped lambda calculus, enhanced with 
+numbers and arithmetic. There are two main challenges with implementing the untyped lambda calculus: 
+the non-termination of evaluation, and capture-avoiding substitution. We cannot address the first 
+here, since our language as it stands does in fact admit unnormalizable terms like
+\<open>App\<^sub>s (Lam\<^sub>s x (App\<^sub>s (Var\<^sub>s x) (Var\<^sub>s x))) (Lam\<^sub>s x (App\<^sub>s (Var\<^sub>s x) (Var\<^sub>s x)))\<close>; after typechecking, we will 
+lower our sights to the simply-typed subset of our language and be able to prove normalization then.
+As for substitution, for now we take the brute-force approach of renaming every binder to a fresh 
+variable every time we substitute past it. We will shortly switch to a nameless Debruijn-index 
+representation to make substitution simpler, but we want to keep out source language as close to an 
+intuitive, "human-readable" version as possible. After all, changing this sort of behaviour to one 
+more easily implemented on a computer is the essence of compilation.\<close>
+
+(* TODO: products and sums *)
+
+datatype expr\<^sub>s = 
+  Var\<^sub>s var
+  | Const\<^sub>s nat
+  | Lam\<^sub>s var expr\<^sub>s
+  | App\<^sub>s expr\<^sub>s expr\<^sub>s
+
+text \<open>Only numbers and lambda-abstractions are values:\<close>
+
+primrec "value" :: "expr\<^sub>s \<Rightarrow> bool" where
+  "value (Var\<^sub>s x) = False"
+| "value (Const\<^sub>s k) = True" 
+| "value (Lam\<^sub>s x e) = True" 
+| "value (App\<^sub>s e\<^sub>1 e\<^sub>2) = False" 
+
+text \<open>Our capture-avoiding substitution requires some helper methods. First, a function to gather up 
+all variables in an expression:\<close>
+
+primrec all_vars :: "expr\<^sub>s \<Rightarrow> var set" where
+  "all_vars (Var\<^sub>s x) = {x}"
+| "all_vars (Const\<^sub>s k) = {}"
+| "all_vars (Lam\<^sub>s x e) = insert x (all_vars e)"
+| "all_vars (App\<^sub>s e\<^sub>1 e\<^sub>2) = all_vars e\<^sub>1 \<union> all_vars e\<^sub>2"
+
+lemma all_vars_finite: "finite (all_vars e)"
+  by (induction e) simp_all
+
+text \<open>Next, we make a limited form of substitution that simply swaps one variable for another. Note 
+that this function is unsafe if the replacement variable is bound in the expression; we will only 
+ever use it in \<open>subst\<close>, where we generate a fresh variable for it.\<close>
+
+primrec subst_var :: "var \<Rightarrow> var \<Rightarrow> expr\<^sub>s \<Rightarrow> expr\<^sub>s" where
+  "subst_var x x' (Var\<^sub>s y) = Var\<^sub>s (if x = y then x' else y)"
+| "subst_var x x' (Const\<^sub>s k) = Const\<^sub>s k"
+| "subst_var x x' (Lam\<^sub>s y e) = Lam\<^sub>s y (if x = y then e else subst_var x x' e)"
+| "subst_var x x' (App\<^sub>s e\<^sub>1 e\<^sub>2) = App\<^sub>s (subst_var x x' e\<^sub>1) (subst_var x x' e\<^sub>2)"
+
+lemma size_subst_var [simp]: "size (subst_var x x' e) = size e"
+  by (induction e) simp_all
+
+text \<open>Finally, our capture-avoiding substitution function. As noted above, we rename every binder 
+every time we pass one, using the \<open>subst_var\<close> helper method to avoid an infinite regress. Indeed, we 
+still need the \<open>size_subst_var\<close> lemma just to prove termination.\<close> 
+
+fun subst\<^sub>s :: "var \<Rightarrow> expr\<^sub>s \<Rightarrow> expr\<^sub>s \<Rightarrow> expr\<^sub>s" where
+  "subst\<^sub>s x e' (Var\<^sub>s y) = (if x = y then e' else Var\<^sub>s y)"
+| "subst\<^sub>s x e' (Const\<^sub>s k) = Const\<^sub>s k"
+| "subst\<^sub>s x e' (Lam\<^sub>s y e) = (
+    let z = fresh (all_vars e' \<union> all_vars e \<union> {x, y})
+    in Lam\<^sub>s z (subst\<^sub>s x e' (subst_var y z e)))"
+| "subst\<^sub>s x e' (App\<^sub>s e\<^sub>1 e\<^sub>2) = App\<^sub>s (subst\<^sub>s x e' e\<^sub>1) (subst\<^sub>s x e' e\<^sub>2)"
+
+text \<open>Now, we define big-step evaluation. It is represented by an inductive relation rather than an
+evaluation function because, of course, some source expressions do not have a normal form. However, 
+even once we prove termination for later stages, we will mostly use an inductive definition of 
+evaluation simply because it is easier to write and work with.\<close> 
+
+inductive eval\<^sub>s :: "expr\<^sub>s \<Rightarrow> expr\<^sub>s \<Rightarrow> bool" (infix "\<Down>" 50) where
+  ev\<^sub>s_const [simp]: "Const\<^sub>s k \<Down> Const\<^sub>s k"
+| ev\<^sub>s_lam [simp]: "Lam\<^sub>s x e \<Down> Lam\<^sub>s x e"
+| ev\<^sub>s_app [simp]: "e\<^sub>1 \<Down> Lam\<^sub>s x e\<^sub>1' \<Longrightarrow> e\<^sub>2 \<Down> v\<^sub>2 \<Longrightarrow> subst\<^sub>s x v\<^sub>2 e\<^sub>1' \<Down> v \<Longrightarrow> App\<^sub>s e\<^sub>1 e\<^sub>2 \<Down> v"
+
+text \<open>Since our language is untyped, we cannot prove (or even express) the progress and preservation 
+theorems. However, we can prove determinism of evaluation:\<close>
+
+theorem determinismn: "e \<Down> v \<Longrightarrow> e \<Down> v' \<Longrightarrow> v = v'"
+proof (induction e v arbitrary: v' rule: eval\<^sub>s.induct)
+  case (ev\<^sub>s_const k)
+  thus ?case by (induction "Const\<^sub>s k" v' rule: eval\<^sub>s.induct) simp_all
+next
+  case (ev\<^sub>s_lam x e)
+  thus ?case by (induction "Lam\<^sub>s x e" v' rule: eval\<^sub>s.induct) simp_all
+next
+  case (ev\<^sub>s_app e\<^sub>1 x e\<^sub>1' e\<^sub>2 v\<^sub>2 v)
+  from ev\<^sub>s_app(7, 1, 2, 3, 4, 5, 6) show ?case 
+    by (induction "App\<^sub>s e\<^sub>1 e\<^sub>2" v' rule: eval\<^sub>s.induct) blast+
+qed
+
+end
